ver2/storage_cmp_impl.v
@@ -44,17 +44,20 @@ Module StorageCmpImpl.
 
 
   Definition sstorage_cmp_t := sstorage -> sstorage -> nat -> sbindings -> nat -> sbindings -> nat -> stack_op_instr_map -> bool.
-(* sstack_val_cmp sstrg1 sstrg2 maxidx1 sb1 maxid2 sb2 instk_height ops -> bool *)
-Definition sstorage_cmp_ext_t := sstack_val_cmp_t -> sstorage_cmp_t.
+
+  (* sstack_val_cmp sstrg1 sstrg2 maxidx1 sb1 maxid2 sb2 instk_height ops -> bool *)
+  Definition sstorage_cmp_ext_t := sstack_val_cmp_t -> sstorage_cmp_t.
 
 
-Definition trivial_storage_cmp (sstack_val_cmp : sstack_val_cmp_t) (sstrg1 sstrg2 :sstorage) (maxidx1: nat) (sb1: sbindings) (maxidx2: nat) (sb2: sbindings) (instk_height: nat) (ops: stack_op_instr_map) : bool :=
+  (* just handles the case of empty storage updates *)
+  Definition trivial_storage_cmp (sstack_val_cmp : sstack_val_cmp_t) (sstrg1 sstrg2 :sstorage) (maxidx1: nat) (sb1: sbindings) (maxidx2: nat) (sb2: sbindings) (instk_height: nat) (ops: stack_op_instr_map) : bool :=
   match sstrg1,sstrg2 with
   | [], [] => true
   | _, _ =>  false
   end.
 
-Fixpoint basic_storage_cmp (sstack_val_cmp : sstack_val_cmp_t) (sstrg1 sstrg2 :sstorage) (maxidx1: nat) (sb1: sbindings) (maxidx2: nat) (sb2: sbindings) (instk_height: nat) (ops: stack_op_instr_map) : bool :=
+  (* identical storage updates *)
+  Fixpoint basic_storage_cmp (sstack_val_cmp : sstack_val_cmp_t) (sstrg1 sstrg2 :sstorage) (maxidx1: nat) (sb1: sbindings) (maxidx2: nat) (sb2: sbindings) (instk_height: nat) (ops: stack_op_instr_map) : bool :=
   match sstrg1,sstrg2 with
   | [], [] => true
   | (U_SSTORE _ skey1 svalue1)::sstrg1', (U_SSTORE _ skey2 svalue2)::sstrg2' =>
@@ -68,7 +71,55 @@ Fixpoint basic_storage_cmp (sstack_val_cmp : sstack_val_cmp_t) (sstrg1 sstrg2 :s
   | _, _ => false
   end.
 
-                                                                                                                                                                                                             
+  
+  Definition swap_storage_update (u1 u2 : storage_update sstack_val) : bool :=
+    match u1, u2 with
+    | U_SSTORE _ (Val v1) _, U_SSTORE _ (Val v2) _ => ((wordToN v2) <? (wordToN v1))%N
+    | _,_ => false                                                             
+    end.
+  
+  Fixpoint reorder_updates' (d : nat) (sstrg :sstorage) : bool * sstorage :=
+    match d with
+    | O => (false,sstrg)
+    | S d' =>
+        match sstrg with
+        | u1::u2::sstrg' =>
+            if swap_storage_update u1 u2 then
+              match reorder_updates' d' (u1::sstrg') with
+                (_,sstrg'') => (true,u2::sstrg'')
+              end
+            else
+              match reorder_updates' d' (u2::sstrg') with
+                (r,sstrg'') => (r,u1::sstrg'')
+              end
+        | _ => (false,sstrg)
+        end
+    end.
+
+  (* n is basically the length of sstrg, we pass it as a parameter to
+  avoid computing *)
+  Fixpoint reorder_storage_updates (d n: nat) (sstrg :sstorage) : sstorage :=
+    match d with
+    | O => sstrg
+    | S d' =>
+        match reorder_updates' n sstrg with
+        |  (changed,sstrg') =>
+             if changed then
+               reorder_storage_updates d' n sstrg'
+             else
+               sstrg'
+        end
+    end.
 
 
+  Definition po_storage_cmp (sstack_val_cmp : sstack_val_cmp_t) (sstrg1 sstrg2 :sstorage) (maxidx1: nat) (sb1: sbindings) (maxidx2: nat) (sb2: sbindings) (instk_height: nat) (ops: stack_op_instr_map) : bool :=
+    let n1 := length sstrg1 in
+    let n2 := length sstrg2 in
+    if (n1 =? n2) then 
+      let sstrg1' := reorder_storage_updates n1 n1 sstrg1 in
+      let sstrg2' := reorder_storage_updates n2 n2 sstrg2 in
+      basic_storage_cmp sstack_val_cmp sstrg1' sstrg2' maxidx1 sb1 maxidx2 sb2 instk_height ops
+    else
+      false.
+      
 End StorageCmpImpl.
