ver2/memory_cmp_impl_soundness.v
@@ -65,6 +65,10 @@ Module MemoryCmpImplSoundness.
   Proof.
   Admitted.
   
+  Theorem po_memory_cmp_snd:
+    safe_smemory_cmp_ext_wrt_sstack_value_cmp po_memory_cmp.
+  Proof.
+  Admitted.
 
 
 End MemoryCmpImplSoundness.
